src/ReactorModel/Objects/Reactor/Hierarchical.lean
@@ -8,13 +8,13 @@ namespace Reactor
 def UniqueIDs [Reactor α] (rtr : α) : Prop :=
   ∀ {cpt i}, Subsingleton (Member cpt i rtr)
 
-class Indexable (α) extends Reactor α where
+class Hierarchical (α) extends Reactor α where
   unique_ids : ∀ {rtr : α}, UniqueIDs rtr
 
-def Indexable.obj? [Indexable α] (rtr : α) (cpt : Component) : cpt.idType ⇀ cpt.type α :=
+def Hierarchical.obj? [Hierarchical α] (rtr : α) (cpt : Component) : cpt.idType ⇀ cpt.type α :=
   fun i => if h : ∃ o, Object rtr cpt i o then h.choose else none
 
-notation (priority := 1001) rtr "[" cpt "]" => Indexable.obj? rtr cpt
-notation rtr "[" cpt "][" i "]"             => Indexable.obj? rtr cpt i 
+notation (priority := 1001) rtr "[" cpt "]" => Hierarchical.obj? rtr cpt
+notation rtr "[" cpt "][" i "]"             => Hierarchical.obj? rtr cpt i 
 
 end Reactor
